src/program_proof/pav/phys_hist.v
@@ -1,101 +1,114 @@
 From Perennial.program_proof.pav Require Import prelude.
-From Goose.github_com.mit_pdos.pav Require Import kt.
+From Goose.github_com.mit_pdos.pav Require Import alicebob.
 
 From Perennial.program_proof.pav Require Import core serde.
 
-Section wps.
+Section proof.
 Context `{!heapGS Σ, !pavG Σ}.
 
-Definition is_HistEntry (ptr : loc) (obj : map_val_ty) : iProp Σ :=
-  ∃ sl_HistVal,
-  "#Hptr_Epoch" ∷ ptr ↦[HistEntry :: "Epoch"]□ #obj.1 ∗
-  "#Hptr_HistVal" ∷ ptr ↦[HistEntry :: "HistVal"]□ (slice_val sl_HistVal) ∗
-  "#Hsl_HistVal" ∷ own_slice_small sl_HistVal byteT DfracDiscarded obj.2.
+Definition is_histEntry (ptr : loc) (opt_pk : option pk_ty) : iProp Σ :=
+  match opt_pk with
+  | None =>
+    "#Hptr_is_reg" ∷ ptr ↦[histEntry :: "isReg"]□ #false
+  | Some pk =>
+    ∃ sl_pk,
+    "#Hptr_is_reg" ∷ ptr ↦[histEntry :: "isReg"]□ #true ∗
+    "#Hptr_pk" ∷ ptr ↦[histEntry :: "pk"]□ (slice_val sl_pk) ∗
+    "#Hsl_pk" ∷ own_slice_small sl_pk byteT DfracDiscarded pk
+  end.
 
 Definition own_hist sl_hist hist : iProp Σ :=
   ∃ dim0_hist,
   "Hsl_hist" ∷ own_slice sl_hist ptrT (DfracOwn 1) dim0_hist ∗
-  "#Hdim0_hist" ∷ ([∗ list] p;o ∈ dim0_hist;hist, is_HistEntry p o).
+  "#Hdim0_hist" ∷ ([∗ list] p;o ∈ dim0_hist;hist, is_histEntry p o).
 
-Lemma wp_put_hist sl_hist hist ptr_e ep pk  :
+Lemma wp_extendHist sl_hist hist (num_epochs : w64) :
   {{{
     "Hown_hist" ∷ own_hist sl_hist hist ∗
-    "#His_entry" ∷ is_HistEntry ptr_e (ep, pk)
+    "%Hlen_epochs" ∷ ⌜ Z.of_nat $ length hist <= uint.Z num_epochs ⌝
   }}}
-  SliceAppend ptrT (slice_val sl_hist) #ptr_e
+  extendHist (slice_val sl_hist) #num_epochs
   {{{
     sl_hist', RET (slice_val sl_hist');
-    "Hown_hist" ∷ own_hist sl_hist' (hist ++ [(ep, pk)])
+    "Hown_hist" ∷ own_hist sl_hist' (hist ++
+      replicate (uint.nat num_epochs - length hist) (mjoin $ last hist))
   }}}.
 Proof.
-  iIntros (Φ) "H HΦ". iNamed "H". iNamed "Hown_hist".
-  wp_apply (wp_SliceAppend with "Hsl_hist"). iIntros (?) "Hsl_hist".
-  iDestruct (big_sepL2_snoc with "[$Hdim0_hist $His_entry]") as "Hnew_dim0_hist".
-  iApply "HΦ". iFrame "∗#".
+  iIntros (Φ) "H HΦ". wp_rec. iNamed "H". iNamed "Hown_hist".
+  wp_apply wp_slice_len.
+  iDestruct (own_slice_sz with "Hsl_hist") as %?.
+  iDestruct (big_sepL2_length with "Hdim0_hist") as %?.
+  wp_apply wp_Assert_decide; [word|].
+
+  wp_apply wp_ref_of_zero; [done|].
+  iIntros "* Hptr2_last".
+  wp_pures. wp_bind (If _ _ _).
+  wp_apply (wp_wand _ _ _
+    (λ _,
+    ∃ (ptr_entry : loc),
+    "Hsl_hist" ∷ own_slice sl_hist ptrT (DfracOwn 1) dim0_hist ∗
+    "Hptr2_last" ∷ l ↦[ptrT] #ptr_entry ∗
+    "#Hentry" ∷ is_histEntry ptr_entry (mjoin $ last hist)
+    )%I
+    with "[Hptr2_last Hsl_hist]"
+  ).
+  { wp_if_destruct.
+    - wp_apply wp_allocStruct; [val_ty|].
+      iIntros "* Hptr_last".
+      wp_store.
+
+      iPersist "Hptr_last".
+      iDestruct (struct_fields_split with "Hptr_last") as "{Hptr_last} #H".
+      iNamed "H".
+      destruct hist. 2: { simpl in *. word. }
+      by iFrame "∗#".
+    - wp_pures.
+      destruct (last hist) eqn:Hlast_hist.
+      2: { apply last_None in Hlast_hist. simplify_eq/=. word. }
+      rewrite last_lookup in Hlast_hist.
+      iDestruct (big_sepL2_lookup_2_some with "Hdim0_hist") as %[??]; [done|].
+      iDestruct (big_sepL2_lookup with "Hdim0_hist") as "His_entry"; [done..|].
+      replace (pred $ length hist) with
+        (uint.nat (word.sub sl_hist.(Slice.sz) (W64 1))) in * by word.
+      iDestruct (own_slice_small_read with "Hsl_hist") as "[Hsl_hist Hclose]".
+      wp_apply (wp_SliceGet with "[$Hsl_hist]"); [done|].
+      iIntros "Hsl_hist".
+      iDestruct ("Hclose" with "Hsl_hist") as "Hsl_hist".
+      wp_store.
+      by iFrame "∗#". }
+
+  iIntros "*". iNamed 1.
+  wp_apply wp_ref_to; [val_ty|].
+  iIntros "* Hptr_new_hist".
+  wp_apply wp_ref_to; [val_ty|].
+  iIntros "* Hptr_i".
+  wp_apply (wp_forUpto
+    (λ i,
+    ∃ sl_hist' dim0_hist',
+    "%Hlt_i" ∷ ⌜ Z.of_nat $ length hist <= uint.Z i ⌝ ∗
+    "Hptr2_last" ∷ l ↦[ptrT] #ptr_entry ∗
+    "Hptr_new_hist" ∷ l0 ↦[slice.T ptrT] (slice_val sl_hist') ∗
+    "Hsl_hist" ∷ own_slice sl_hist' ptrT (DfracOwn 1) dim0_hist' ∗
+    "#Hdim0_hist" ∷ ([∗ list] p;o ∈ dim0_hist';(hist ++
+      replicate (uint.nat i - length hist) (mjoin (last hist))),
+      is_histEntry p o)
+    )%I
+    with "[] [$Hptr_i $Hptr2_last $Hptr_new_hist $Hsl_hist]"
+  ); [word|..].
+  2: { replace (_ - _)%nat with (0%nat) by word.
+    list_simplifier. iFrame "#". word. }
+  { iClear "% Hdim0_hist". iIntros (? Φ) "!> (H & Hptr_i & %) HΦ".
+    iNamed "H". do 2 wp_load.
+    wp_apply (wp_SliceAppend with "Hsl_hist").
+    iIntros "* Hsl_hist". wp_store.
+    iApply "HΦ". iFrame.
+    remember (_ - _)%nat as prev_len.
+    replace (_ - _)%nat with (S prev_len) by word.
+    rewrite replicate_S_end (assoc (++)).
+    iFrame "#". iIntros "!>". iSplit; [word|done]. }
+  iClear "#". iIntros "[H _]". iNamed "H".
+  wp_load.
+  iApply "HΦ". by iFrame "∗#".
 Qed.
 
-Lemma wp_GetHist sl_hist hist (ep : w64) :
-  {{{
-    "Hown_hist" ∷ own_hist sl_hist hist
-  }}}
-  GetHist (slice_val sl_hist) #ep
-  {{{
-    (is_reg : bool) sl_pk pk, RET (#is_reg, slice_val sl_pk);
-    "Hown_hist" ∷ own_hist sl_hist hist ∗
-    "#Hsl_pk" ∷ own_slice_small sl_pk byteT DfracDiscarded pk ∗
-    "%Heq_lat" ∷
-      ⌜ match lookup_puts_hist hist ep with
-        | None => is_reg = false
-        | Some pk' => is_reg = true ∧ pk = pk'
-        end ⌝
-  }}}.
-Proof.
-  iIntros (Φ) "H HΦ". iNamed "H". rewrite /GetHist. iNamed "Hown_hist".
-  wp_apply wp_ref_of_zero; [done|]. iIntros (ptr_isReg) "Hptr_isReg".
-  wp_apply wp_ref_of_zero; [done|]. iIntros (ptr_val) "Hptr_val".
-  iDestruct (own_slice_small_read with "Hsl_hist") as "[Hsl_hist Hsl_restore]".
-  wp_apply (wp_forSlicePrefix
-    (λ donel _,
-    ∃ (is_reg : bool) sl_pk pk,
-    "Hptr_isReg" ∷ ptr_isReg ↦[boolT] #is_reg ∗
-    "Hptr_val" ∷ ptr_val ↦[slice.T byteT] (slice_val sl_pk) ∗
-    "Hsl_pk" ∷ own_slice_small sl_pk byteT DfracDiscarded pk ∗
-    "%Heq_lat" ∷
-      ⌜ match lookup_puts_hist (take (length donel) hist) ep with
-        | None => is_reg = false
-        | Some pk' => is_reg = true ∧ pk = pk'
-        end ⌝)%I with "[] [$Hsl_hist Hptr_isReg Hptr_val]").
-  2: { iExists _, Slice.nil, []. iFrame. iSplit; [|done].
-    iDestruct (own_slice_zero byteT) as "H".
-    by iDestruct (own_slice_to_small with "H") as "?". }
-  { clear. iIntros "* %". iIntros (Φ) "!> H HΦ". iNamed "H".
-    opose proof (list_lookup_middle done todo x _ _) as Hlook_x; [done|].
-    subst dim0_hist.
-    iDestruct (big_sepL2_lookup_1_some with "Hdim0_hist")
-      as %[[new_ep new_pk] Hlook_hist]; [exact Hlook_x|].
-    iDestruct (big_sepL2_lookup with "Hdim0_hist")
-      as "His_entry"; [exact Hlook_x|exact Hlook_hist|].
-    iNamed "His_entry". wp_loadField. wp_if_destruct.
-    - wp_store. wp_loadField. wp_store. iApply "HΦ".
-      iFrame "Hsl_HistVal". iFrame "∗#". rewrite app_length. simpl.
-      replace (length done + 1)%nat with (S $ length done)%nat; [|lia].
-      rewrite (take_S_r _ _ _ Hlook_hist).
-      rewrite /lookup_puts_hist filter_app.
-      opose proof (list_filter_singleton (λ x, uint.Z x.1 ≤ uint.Z ep)
-        (new_ep, new_pk)) as [[_?]|[Htmp _]]. { exfalso. simpl in *. word. }
-      rewrite Htmp. clear Htmp. rewrite last_snoc. naive_solver.
-    - iApply "HΦ". iFrame "Hsl_pk". iFrame "∗#". rewrite app_length. simpl.
-      replace (length done + 1)%nat with (S $ length done)%nat; [|lia].
-      rewrite (take_S_r _ _ _ Hlook_hist).
-      rewrite /lookup_puts_hist filter_app.
-      opose proof (list_filter_singleton (λ x, uint.Z x.1 ≤ uint.Z ep)
-        (new_ep, new_pk)) as [[Htmp _]|[_?]]. 2: { exfalso. simpl in *. word. }
-      rewrite Htmp. clear Htmp. list_simplifier. by iFrame "%". }
-  iIntros "[H0 H1]". iNamed "H1". iDestruct ("Hsl_restore" with "H0") as "Hsl_hist".
-  do 2 wp_load. wp_pures. iApply "HΦ". iFrame "∗#".
-  iDestruct (big_sepL2_length with "Hdim0_hist") as %Htmp.
-  rewrite Htmp in Heq_lat. clear Htmp.
-  rewrite firstn_all in Heq_lat. naive_solver.
-Qed.
-
-End wps.
+End proof.
